coq: STLC

coq/Logic/STLC/Typing2.v
@@ -1,3 +1,6 @@
+(* This module only serves to demonstrate that defining the typing relation     *)
+(* with stronger requirements in terms of context validity and well-formedness  *)
+(* of type expressions is unnecessary and yields an equivalent notion.          *)
 Require Import Logic.Class.Eq.
 
 Require Import Logic.STLC.Valid.
@@ -7,28 +10,91 @@ Require Import Logic.STLC.Typing.
 Require Import Logic.STLC.Context.
 
 Inductive Judgement2 (b v:Type) (eq:Eq v): Context -> Typing -> Prop :=
-| JAnn : forall (G:Context) (e:Exp b v) (Ty:T b),
+| JAnn2 : forall (G:Context) (e:Exp b v) (Ty:T b),
     Valid G                                     ->  (* superfluous              *)
     G :> Ty                                     ->  (* superfluous              *)
     Judgement2 b v eq G (e >: Ty)               ->
     Judgement2 b v eq G ((e :: Ty) >: Ty)    
-| JVar : forall (G:Context) (x:v) (Ty:T b),
+| JVar2 : forall (G:Context) (x:v) (Ty:T b),
     Valid G                                     -> 
     G :> Ty                                     ->  (* superfluous              *)
     G :>> x ::: Ty                              -> 
     Judgement2 b v eq G (`x >: Ty)            
-| JApp : forall (G:Context) (e1 e2:Exp b v) (Ty Ty':T b),
+| JApp2 : forall (G:Context) (e1 e2:Exp b v) (Ty Ty':T b),
     Valid G                                     ->  (* superfluous              *)
     G :> Ty                                     ->  (* superfluous              *)
     G :> Ty'                                    ->  (* superfluous              *)
     Judgement2 b v eq G (e1 >: Ty :-> Ty')      ->  
     Judgement2 b v eq G (e2 >: Ty)              -> 
     Judgement2 b v eq G (e1 $ e2 >: Ty')        
-| JLam : forall (G:Context) (x:v) (e:Exp b v) (Ty Ty':T b),
+| JLam2 : forall (G:Context) (x:v) (e:Exp b v) (Ty Ty':T b),
     Valid G                                     ->  
     G :> Ty                                     ->  
     Judgement2 b v eq (G;x ::: Ty) (e >: Ty')   ->  
     Judgement2 b v eq G ((\x ~> e) >: Ty :-> Ty')
 .
 
+Arguments Judgement2 {b} {v} {eq}.
+Arguments JAnn2      {b} {v} {eq}.
+Arguments JVar2      {b} {v} {eq}.
+Arguments JApp2      {b} {v} {eq}.
+Arguments JLam2      {b} {v} {eq}.
 
+(* Building a proof of Judgment2 requires more evidence that for building a     *)
+(* proof of Judgment. Hence expecting the following implication to hold.        *)
+Lemma Judgement2Judgement : 
+    forall (b v:Type) (eq:Eq v) (G:Context) (e:Exp b v) (Ty:T b),
+        Judgement2 G (e >: Ty) -> G :- e >: Ty.
+Proof.
+    intros b v eq G e Ty H1. remember (e >: Ty) as k eqn:E. revert e Ty E.
+    induction H1 as 
+        [ G e Ty H2 H3 H4 IH
+        | G x Ty H2 H3 H4  
+        | G e1 e2 Ty Ty' H2 H3 H4 H5 IH1 H6 IH2
+        | G x e Ty Ty' H2 H3 H4 IH 
+        ]; intros e' Sy H7; inversion H7; subst; clear H7. 
+    - apply JAnn. apply IH with e Sy. reflexivity.
+    - apply JVar; assumption.
+    - apply JApp with Ty.
+        + apply IH1 with e1 (Ty :-> Sy). reflexivity.
+        + apply IH2 with e2 Ty. reflexivity.
+    - apply JLam; try assumption. apply IH with e Ty'. reflexivity.
+Qed.
+
+
+(* However, we know that a Judgement cannot hold unless the context is valid    *)
+(* and the type expression is well-formed. So the following should hold.        *)
+ Lemma JudgementJudgement2 : 
+    forall (b v:Type) (eq:Eq v) (G:Context) (e:Exp b v) (Ty:T b),
+        G :- e >: Ty -> Judgement2 G (e >: Ty).
+Proof.
+    intros b v eq G e Ty H1. remember (e >: Ty) as k eqn:E. revert e Ty E.
+    induction H1 as
+        [ G e Ty H2 IH
+        | G x Ty H2 H3 
+        | G e1 e2 Ty Ty' H2 IH1 H3 IH2
+        | G x e Ty Ty' H2 H3 H4 IH 
+        ]; intros e' Sy H7; inversion H7; subst; clear H7. 
+    - apply JAnn2.
+        + apply TypedIsValid with eq e Sy. assumption.
+        + apply TypedIsType with eq e. assumption.
+        + apply IH with e Sy. reflexivity.
+    - apply JVar2; try assumption. apply ValidIsType with eq x; assumption.
+    - apply JApp2 with Ty.
+        + apply TypedIsValid with eq e2 Ty. assumption.
+        + apply TypedIsType with eq e2. assumption.
+        + apply IsTypeRevR with Ty. apply TypedIsType with eq e1. assumption.
+        + apply IH1 with e1 (Ty :-> Sy). reflexivity.
+        + apply IH2 with e2 Ty. reflexivity.
+    - apply JLam2; try assumption. apply IH with e Ty'. reflexivity.
+Qed.
+
+(* This vindicates our streamlined definition of the Judgement predicate.       *)
+Theorem JudgementJudgement2Same:
+    forall (b v:Type) (eq:Eq v) (G:Context) (e:Exp b v) (Ty:T b),
+        G :- e >: Ty <-> Judgement2 G (e >: Ty).
+Proof.
+    intros b v eq G e Ty. split; intros H1.
+    - apply JudgementJudgement2. assumption.
+    - apply Judgement2Judgement. assumption.
+Qed.
